theories/goedel/fixPoint.v
@@ -241,7 +241,7 @@ Proof.
         | H:(In ?X3 (freeVarFormula LNN (andH ?X1 ?X2))) |- _ =>
             assert (In X3 (freeVarFormula LNN X1 ++ freeVarFormula LNN X2));
             [ apply H | clear H ]
-        | H:(In ?X3 (freeVarFormula LNN (fol.impH LNN ?X1 ?X2))) |- _ =>
+        | H:(In ?X3 (freeVarFormula LNN (impH LNN ?X1 ?X2))) |- _ =>
             assert (In X3 (freeVarFormula LNN X1 ++ freeVarFormula LNN X2));
             [ apply H | clear H ]
         | H:(In ?X3 (freeVarFormula LNN (fol.notH LNN ?X1))) |- _ =>
@@ -576,7 +576,7 @@ Proof.
         | H:(In ?X3 (freeVarFormula LNT (andH  ?X1 ?X2))) |- _ =>
             assert (In X3 (freeVarFormula LNT X1 ++ freeVarFormula LNT X2));
             [ apply H | clear H ]
-        | H:(In ?X3 (freeVarFormula LNT (fol.impH LNT ?X1 ?X2))) |- _ =>
+        | H:(In ?X3 (freeVarFormula LNT (impH LNT ?X1 ?X2))) |- _ =>
             assert (In X3 (freeVarFormula LNT X1 ++ freeVarFormula LNT X2));
             [ apply H | clear H ]
         | H:(In ?X3 (freeVarFormula LNT (fol.notH LNT ?X1))) |- _ =>
